Some progress on proof; stuck on binary expressions and calls/invocations

proof_of_soundness/Transformations.v
@@ -28,87 +28,120 @@ Inductive TransformExpr :
     TransformExpr M F e0 F' e0' ->
     TransformExpr M F (UnExpr uo e0) F' (UnExpr uo e0')
   
-  | Transform_BinExpr : forall M F e1 e2 F' F'' F''' e1' e2' bo,
+  | Transform_BinExpr : forall M F e1 e2 F' F'' e1' e2' bo,
     TransformExpr M F e1 F' e1' ->
     TransformExpr M F e2 F'' e2' ->
-    
-    (* Note that we don't explicity create F''' here. In the implementation, F''' will
-       be created as the the unification of F' and F''. *)
-    (* We need these extra theorems until we resolve the unique names problem, but
-       these should make sense for now*)
-    (* If we can evaluate the left expression under its F transformation, then we can
-       evaluate it under the unified F list *)
-    (forall S E G v S',
-      ExprEval S E G F' M e1' v S' -> ExprEval S E G F''' M e1' v S') ->
-    (* Similarly, if we can evaluate the right expression under its F transformation,
-       then we can evaluate it under the unified F list as well *)
-    (forall S'0 E G v2 S',
-      ExprEval S'0 E G F'' M e2' v2 S' -> ExprEval S'0 E G F''' M e2' v2 S') ->
-    TransformExpr M F (BinExpr bo e1 e2) F''' (BinExpr bo e1' e2')
-    
-    | Transform_Assign : forall M F x e F' e',
-      TransformExpr M F e F' e' ->
-      TransformExpr M F (Assign x e) F' (Assign x e')
+    (* If an expression is evaluable under F', then it should be evaluable under F'' *)
+    (* There may be a better way to prove this, but I can't figure out how to do it yet *)
+    (forall S E G v S', ExprEval S E G F' M e1' v S' -> ExprEval S E G F'' M e1' v S') ->
+    TransformExpr M F (BinExpr bo e1 e2) F'' (BinExpr bo e1' e2')
+  
+  | Transform_Assign : forall M F x e F' e',
+    TransformExpr M F e F' e' ->
+    TransformExpr M F (Assign x e) F' (Assign x e')
 
-    | Transform_FunctionCall : forall F M x es,
-      (* Macros shadow functions, so to determine if what we are calling is a function
-         it suffices just to check that its name is not in the macro table and is in
-         the function table *)
-      ~ StringMap.In x M ->
-      StringMap.In x F ->
-      (* TODO: Transform function arguments *)
-      TransformExpr M F (CallOrInvocation x es) F (CallOrInvocation x es)
-      
-    | Transform_SideEffectFreeMacro :
-      forall  F M x es F' params mexpr fname
-              (vs : list Z) (ls : list nat) (Ef : environment)
-              (Sargs : store) (S'' : store) (S''' : store) (S'''' : store)
-              (S''''' : store),
-      (* Again, macros shadow functions, so we just have to check if the callee's name
-         is in the macro table to determine if it is a macro. *)
-      
-      StringMap.In x M ->
-      
-      (* Assert that there is only one mapping for x in the macro table *)
-      (forall params' mexpr',
-        StringMap.MapsTo x (params', mexpr') M -> params' = params /\ mexpr' = mexpr) ->
-      
-      (* The macro does not have side-effects *)
-      ~ ExprHasSideEffects mexpr ->
-      Forall (fun e => ~ ExprHasSideEffects e) es ->
-      
-      (* The name for transformed macro function is not already present in the function
-         table *)
-      ~ StringMap.In fname F ->
-      StringMap.Equal F' (StringMap.add fname (params, Skip, mexpr) F) ->
-      
-      
-      (* TODO: Transform macro arguments *)
-      
-      
-      (* We need to manually add all the premises for function calls that we can't
-         intuit from the proof context alone, because macro invocation just doesn't do
-         certain things that function calls do, such as evaluating arguments in an
-         eager manner *)
+  | Transform_FunctionCall :
+    forall   F M x es F' F'' F''' F'''' es'
+             params fstmt fexpr fstmt' fexpr',
+    (* Macros shadow functions, so to determine if what we are calling is a function
+       it suffices just to check that its name is not in the macro table and is in
+       the function table *)
+    ~ StringMap.In x M ->
+    StringMap.MapsTo x (params, fstmt, fexpr) F ->
+    
+    (* There is only one mapping for x in the original function table *)
+    (forall params0 fstmt0 fexpr0 params1 fstmt1 fexpr1,
+      StringMap.MapsTo x (params0, fstmt0, fexpr0) F ->
+      (params0, fstmt0, fexpr0) = (params1, fstmt1, fexpr1)) ->
+    
+    (* Transform function arguments first *)
+    TransformArgs M F es F' es' ->
+    TransformStmt M F' fstmt F'' fstmt' ->
+    TransformExpr M F'' fexpr F''' fexpr' ->
+    StringMap.Equal F'''' (StringMap.add x (params, fstmt', fexpr') F''') ->
+    TransformExpr M F (CallOrInvocation x es) F'''' (CallOrInvocation x es')
+    
+  | Transform_SideEffectFreeMacro :
+    forall  F M x es F' F'' es' params mexpr fname
+  
+          (S : store) (E : environment) (G : environment)
+          (vs : list Z) (ls : list nat) (v : Z) (Ef : environment)
+          Sargs S' S'' S''' S'''' S''''',
+    (* Again, macros shadow functions, so we just have to check if the callee's name
+       is in the macro table to determine if it is a macro. *)
+    
+    StringMap.MapsTo x (params, mexpr) M ->
+    
+    (* There is only one mapping for x in the macro table *)
+    (forall params0 mexpr0 params1 mexpr1,
+      StringMap.MapsTo x (params0, mexpr0) M ->
+      (params0, mexpr0) = (params1, mexpr1) ) ->
+    
+    (* The macro does not have side-effects *)
+    ~ ExprHasSideEffects mexpr ->
+    Forall (fun e => ~ ExprHasSideEffects e) es ->
+    
+    (* Transform macro arguments first *)
+    TransformArgs M F es F' es' ->
+    
+    (* Add the transformed function definition to the function table *)
+    ~ StringMap.In fname F' ->
+    StringMap.Equal F'' (StringMap.add fname (params, Skip, mexpr) F') ->
+    
+    
+    
+    
+    (* We need to manually add all the premises for function calls that we can't
+       intuit from the proof context alone, because macro invocation just doesn't do
+       certain things that function calls do, such as evaluating arguments in an
+       eager manner *)
+    (* These premises are currently too lenient though; we should only use the original
+       F in these and prove that they will still hold under F'' *)
        ~ StringMap.In fname M ->
       (* StringMap.MapsTo x (params, fstmt, fexpr) F /\ *) (* We can prove this *)
       (* NoDup params /\ *) (* This is given from the macro invocation *)
-      (forall (S : store) (E : environment) (G : environment)
-              (vs : list Z) (ls : list nat) (v : Z) (Ef : environment)
-              Sargs S' S'' S''' S'''' S''''',
-      EvalArgs S E G F' M es vs S' /\
-      StringMap.Equal Ef (StringMapProperties.of_list (combine params ls)) /\
-      NatMap.Equal Sargs (NatMapProperties.of_list (combine ls vs)) /\
-      NatMapProperties.Disjoint S' Sargs /\
-      NatMap.Equal S'' (NatMapProperties.update S' Sargs) /\
-      StmtEval S'' Ef G F' M Skip S''' /\
-      (* Not sure if this is too generous a premise? *)
-      ExprEval S''' Ef G F' M mexpr v S'''' /\
-      (* Only keep in the store the L-value mappings that were there when
-         the function was called; i.e., remove from the store all mappings
-         whose L-value is in Ef/Sargs. *)
-      NatMap.Equal S''''' (NatMapProperties.restrict S'''' S)) ->
-      
-      
-      TransformExpr M F (CallOrInvocation x es) F' (CallOrInvocation fname es).
+      EvalArgs S E G F M es vs S' ->
+      StringMap.Equal Ef (StringMapProperties.of_list (combine params ls)) ->
+      NatMap.Equal Sargs (NatMapProperties.of_list (combine ls vs)) ->
+      NatMapProperties.Disjoint S' Sargs ->
+      NatMap.Equal S'' (NatMapProperties.update S' Sargs) ->
+      StmtEval S'' Ef G F M Skip S''' ->
+      ExprEval S''' Ef G F M mexpr v S'''' ->
+      NatMap.Equal S''''' (NatMapProperties.restrict S'''' S) ->
+    
+    
+    TransformExpr M F (CallOrInvocation x es) F'' (CallOrInvocation fname es)
+with TransformArgs :
+  macro_table -> function_table -> list expr ->
+  function_table -> list expr -> Prop :=
+  
+  (* End of arguments *)
+  | TransformArgs_Nil : forall M F es,
+    TransformArgs M F nil F es
+  
+  (* There are arguments left to transform *)
+  | TransformArgs_Cons : forall M F e es F' F'' e' es',
+    (* Transform the first expression *)
+    TransformExpr M F e F' e' ->
+    (* Transform the remaining expressions *)
+    TransformArgs M F' es F'' es' ->
+    TransformArgs M F (e::es) F'' (e'::es')
+with TransformStmt :
+  macro_table -> function_table -> stmt ->
+  function_table -> stmt -> Prop :=
+  
+  | Transform_Skip : forall M F,
+    TransformStmt M F Skip F Skip.
+
+
+
+
+
+
+
+
+
+
+
+
 
